

$$\boxed{\rho = \frac{p_0}{J}}$$

$$\Leftrightarrow \underline{\underline{M := \rho J}}$$

$$\dot{M} = 0 \quad \Leftrightarrow \quad M \Big|_{T_0} = \text{const.}$$

$$(fJ)' = (p_t + \nabla \cdot (p u)) \Big|_{x_0} \Leftrightarrow p_t + \nabla \cdot (p u) = 0$$

How about $\dot{M} \neq 0$? e.g. Mass-action?

$$\rho_t + \nabla \cdot (\rho \vec{u}) = \underline{\underline{\sum \dot{r}}}$$

Kinematics: $\rho = \rho_0 + \sum \vec{R}$

$$M := \underline{m(t)} = \int_{\Omega} \rho(x, t) dx \stackrel{\text{c.v.t.}}{=} \int_{\underline{\Omega}} \underbrace{\rho(x(\underline{x}, t), t)}_{\text{III}} \left| \frac{\partial x}{\partial \underline{x}} \right| d\underline{x}$$

if III $\quad x = x(\underline{x}, t) \quad \quad \rho(x, t), T(x, t)$

$m|_{t=0}$

$$\int_{\Omega_{\vec{x}}} \rho(\vec{x}, 0) d\vec{x}$$

$\rho(\vec{x}) \leftarrow \rho_0$

$$\rho = \frac{\rho_0}{J}$$

$$\rho = \rho_0 + \sum \vec{R}$$

$$m(t) = \int_{\Omega} \rho(x, t) dx = \int_{\Omega_{\vec{x}}} \rho_0(\vec{x}) + \sum \vec{R}(t, \vec{R}) d\vec{x}$$

$\downarrow \frac{d}{dt} \qquad \qquad \qquad \downarrow \frac{d}{dt}$

$$\int_{\Omega_{\vec{x}}} (\rho_t + \nabla \cdot (\rho u)) J d\vec{x}$$

$$\int_{\Omega_{\vec{x}}} \sum \vec{r} d\vec{x}$$

$$= \int_{\Omega} \rho_t + \nabla \cdot (\rho u) dx$$

$$\int_{\Omega} \sum \vec{r} dx$$

$$\rho_t + \nabla \cdot (\rho u) = \sum \vec{r}, \quad \vec{r} = \vec{r}(\vec{p})$$

eg: $\vec{p} = \begin{bmatrix} B \\ R \\ E \end{bmatrix}$

$\vec{u}_B \equiv \vec{u}_R \equiv \vec{u}_E = 0. \quad (\text{ODE})$

? $\vec{r} = \vec{r}_m(p)$ $\neq \vec{u} = \vec{u}_m(p)$

$\dot{B} = \left(r B (1 - \frac{B}{K}) \right) = r B - \frac{r}{K} B^2$

For $n = 0, 1, 2, \dots$

$B \frac{k_+}{k_-} \geq B$

$u^{n+1} = \vec{u}_m(p^n)$

$\dot{B}^{(n+1)} = (k_+ B - k_- B^2)$

$y_1^{n+1} = \gamma_{1,m}^n (\vec{p}^n)$

$R_1^{n+1} = R_1^n + \text{rot} \left(\gamma_{1,m}^n \right)$

$J^{n+1} = J^n + \text{rot} (\nabla \cdot u) J^n - \underline{u \cdot \nabla J}$

$p^{n+1} = \frac{f_0 + R_1^{n+1}}{J^{n+1}}$

$$\underline{f_t = \Delta p} + \underline{k^+ p - k^- p^2}$$

$$\underline{x_t \approx \frac{x^{n+1} - x^1}{\Delta t} \approx u}$$

$$R_t = \frac{R^{n+1} - R^1}{\Delta t} \approx r_{NN}$$

$$\frac{\partial}{\partial t} r(p)$$

$$\underline{R(t_{\infty}) = 0.}$$

$$V_{FINN}$$

Wei :

$$\underline{p_t = \Delta p + p - p^2}$$

$$p|_{t=0} = p_0$$